working proof, fix findNext spec, some cleanup

coupling_inv.v
@@ -1,5 +1,6 @@
 (** Verification of lock coupling template algorithm *)
 
+Require Import lock.
 From iris.algebra Require Import excl auth gmap agree gset.
 From iris.heap_lang Require Export lifting notation locations lang.
 From iris.base_logic.lib Require Export invariants.
@@ -9,7 +10,7 @@ From iris.heap_lang Require Import proofmode notation par.
 From iris.bi.lib Require Import fractional.
 From iris.bi Require Import derived_laws_sbi.
 Set Default Proof Using "All".
-Require Export keyset_ra inset_flows ccm flows.
+Require Export inset_flows.
 Require Import auth_ext.
 
 (** We use integers as keys. *)
@@ -34,10 +35,7 @@ Section Coupling_Cameras.
   Proof. solve_inG. Qed.
 
   (* RA for pair of keysets and contents *)
-  Class keysetG Σ := KeysetG { keyset_inG :> inG Σ (authUR (keysetUR K)) }.
-  Definition keysetΣ : gFunctors := #[GFunctor (authUR (keysetUR K))].
-
-  Instance subG_keysetΣ {Σ} : subG keysetΣ Σ → keysetG Σ.
+  Instance subG_keysetΣ {Σ} : subG (@keysetΣ K _ _) Σ → (@keysetG K _ _) Σ.
   Proof. solve_inG. Qed.
 
   (* RA for set of contents *)
@@ -51,12 +49,10 @@ End Coupling_Cameras.
 (** Verification of the template *)
 Section Coupling_Template.
 
-  Context `{!heapG Σ, !flowintG Σ, !nodesetG Σ, !keysetG Σ, !contentG Σ} (N : namespace).
+  Context `{!heapG Σ, !flowintG Σ, !nodesetG Σ, !(@keysetG K _ _) Σ, !contentG Σ} (N : namespace).
   Notation iProp := (iProp Σ).
 
   (** The code of the coupling template. *)
-
-  Inductive dOp := searchOp | insertOp | deleteOp.
 
   (* The following parameters are the implementation-specific helper functions
    * assumed by the template. See GRASShopper files b+-tree.spl and
@@ -64,21 +60,7 @@ Section Coupling_Template.
 
   Parameter findNext : val.
   Parameter decisiveOp : (dOp → val).
-  Parameter lockLoc : Node → loc.
-  Parameter getLockLoc : val.
   Parameter alloc : val.
-
-  Definition lockNode : val :=
-    rec: "lockN" "x" :=
-      let: "l" := getLockLoc "x" in
-      if: CAS "l" #false #true
-      then #()
-      else "lockN" "x".
-
-  Definition unlockNode : val :=
-    λ: "x",
-    let: "l" := getLockLoc "x" in
-    "l" <- #false.
 
   Definition traverse : val :=
     rec: "tr" "p" "n" "k" :=
@@ -109,20 +91,15 @@ Section Coupling_Template.
 
   (* The node predicate is specific to each template implementation. *)
   Parameter node : Node → Node → inset_flowint_ur K → gset K → iProp.
-  (* TODO change node n root I C → node root n I C*)
 
   (* The following assumption is justified by the fact that GRASShopper uses a
    * first-order separation logic. *)
-  Parameter node_timeless_proof : ∀ n root I C, Timeless (node n root I C).
-  Instance node_timeless n root I C: Timeless (node n root I C).
+  Parameter node_timeless_proof : ∀ root n I C, Timeless (node root n I C).
+  Instance node_timeless root n I C: Timeless (node root n I C).
   Proof. apply node_timeless_proof. Qed.
 
   (* Spatial part of node predicate. *)
   Parameter hrep_spatial : Node → iProp.
-
-
-  (* TODO: can we get rid of the following? *)
-  Instance ccm_ms : CCM (@K_multiset K _ _) := @K_multiset_ccm K _ _.
 
   (* The node-local invariant. 
    * See list-coupling.spl for the corresponding GRASShopper definition.*)
@@ -135,12 +112,12 @@ Section Coupling_Template.
 
   (* The following hypotheses are proved as GRASShopper lemmas in
    * list-coupling.spl *)
-  Hypothesis node_implies_nodeinv : ∀ n I_n C root,
-    (⌜✓I_n⌝)%I ∗ node n root I_n C
-    -∗ node n root I_n C ∗ (⌜nodeinv root n I_n C⌝)%I.
+  Hypothesis node_implies_nodeinv : ∀ root n I_n C,
+    (⌜✓I_n⌝)%I ∗ node root n I_n C
+    -∗ node root n I_n C ∗ (⌜nodeinv root n I_n C⌝)%I.
 
-  Hypothesis node_sep_star: ∀ n I_n I_n' C C' root,
-    node n root I_n C ∗ node n root I_n' C' -∗ False.
+  Hypothesis node_sep_star: ∀ root n I_n I_n' C C',
+    node root n I_n C ∗ node root n I_n' C' -∗ False.
 
   Lemma successor_not_root : ∀ (I I1 I2 I3 : flowintT) C root n k,
       globalinv K root I →
@@ -168,7 +145,7 @@ Section Coupling_Template.
     unfold cmra_op, flowintRA, cmra_car, K_multiset at 5, K_multiset at 5 in n_inf_I23.
     pose proof (I_inf_out root) as (root_out & _).
     assert (root = root) by reflexivity.
-    pose proof (root_out H k) as root_out_k.
+    pose proof (root_out H0 k) as root_out_k.
 
     assert (default 0 (inf I n !! k) ≠ 0).
     rewrite e.
@@ -185,7 +162,7 @@ Section Coupling_Template.
     rewrite root_out_k.
     simpl in H0.
     simpl.
-    naive_solver.
+    naive_solver. done.
     pose proof (lookup_op _ _ (inf I n) (out I1 n) k) as inf_I23_def.
 
     rewrite IDef in inf_I23_def.
@@ -231,54 +208,38 @@ Section Coupling_Template.
     rewrite <- Heqx1 in inf_I2_def.
     lia.
     all: trivial.
-  Qed.
-
-  (** Coarse-grained specification *)
-
-  Definition Ψ dop k (C: gsetO K) (C': gsetO K) (res: bool) : Prop :=
-    match dop with
-    | searchOp => C' = C ∧ if res then k ∈ C else k ∉ C
-    | insertOp => C' = union C {[k]} ∧ if res then k ∉ C else k ∈ C
-    | deleteOp => C' = difference C {[k]} ∧ if res then k ∈ C else k ∉ C
-    end.
-
+  Qed.  
 
 
   (** Helper functions specs *)
 
-  (* Sid: we can also try to get rid of getLockLoc and just do CAS (lockLoc "l") #true #false in lock, etc. *)
-  Parameter getLockLoc_spec : ∀ (n: Node),
-      ({{{ True }}}
-           getLockLoc #n
-       {{{ (l:loc), RET #l; ⌜lockLoc n = l⌝ }}})%I.
-
   (* The following functions are proved for each implementation in GRASShopper
    * (see list-coupling.spl) *)
 
+  (* TODO ghp spec doesn't match *)
   Parameter findNext_spec : ∀ root (n: Node) (I_n : inset_flowint_ur K) (C: gset K) (k: K),
-      ({{{ node n root I_n C ∗ ⌜in_inset K k I_n n⌝ }}}
+     ⊢ ({{{ node root n I_n C ∗ ⌜in_inset K k I_n n⌝ }}}                
            findNext #n #k
        {{{ (b: bool) (n': Node),
               RET (match b with true => (SOMEV #n') | false => NONEV end);
-               node n root I_n C ∗ (match b with true => ⌜in_outset K k I_n n'⌝ |
+               node root n I_n C ∗ (match b with true => ⌜in_outset K k I_n n'⌝ |
                                           false => ⌜¬in_outsets K k I_n⌝ ∗ ⌜n ≠ root⌝ end) }}})%I.
 
   Parameter decisiveOp_insert_spec : ∀ dop root (p n m: Node) (k: K) (I_p I_n: inset_flowint_ur K) (C_p C_n: gset K),
-      ({{{ node p root I_p C_p ∗ node n root I_n C_n ∗ hrep_spatial m ∗ ⌜n ≠ root⌝ ∗ ⌜m ≠ root⌝
+     ⊢ ({{{ node root p I_p C_p ∗ node root n I_n C_n ∗ hrep_spatial m ∗ ⌜n ≠ root⌝ ∗ ⌜m ≠ root⌝
                           ∗ ⌜in_inset K k I_p p⌝ ∗ ⌜in_outset K k I_p n ⌝ ∗ ⌜¬in_outsets K k I_n⌝ }}}
            decisiveOp dop #p #n #k
        {{{ (C_p' C_n' C_m': gset K) (I_p' I_n' I_m': flowintUR K_multiset) (res: bool), RET  #res;
-                           node p root I_p' C_p' ∗ node n root I_n' C_n' ∗ node m root I_m' C_m'
-                         ∗ ⌜Ψ dop k (C_p ∪ C_n) (C_p' ∪ C_n' ∪ C_m') res⌝
+                           node root p I_p' C_p' ∗ node root n I_n' C_n' ∗ node root m I_m' C_m'
+                         ∗ Ψ dop k (C_p ∪ C_n) (C_p' ∪ C_n' ∪ C_m') res
                          ∗ ⌜contextualLeq _ (I_p ⋅ I_n) (I_p' ⋅ I_n' ⋅ I_m')⌝ ∗ ⌜inf (I_p'⋅I_n'⋅I_m') m = 0%CCM⌝
                          ∗ ⌜domm I_p' = {[p]}⌝ ∗ ⌜domm I_n' = {[n]}⌝ ∗ ⌜domm I_m' = {[m]}⌝
-                         ∗ ⌜C_p' ⊆ keyset K I_p' p⌝ ∗ ⌜C_n' ⊆ keyset K I_n' n⌝ ∗ ⌜C_m' ⊆ keyset K I_m' m⌝
                          ∗ ⌜keyset K I_p' p ## keyset K I_n' n⌝ ∗ ⌜keyset K I_p' p ## keyset K I_m' m⌝
-                         ∗ ⌜keyset K I_m' m ## keyset K I_n' n⌝ ∗ ⌜C_p' ## C_n'⌝ ∗ ⌜C_m' ## C_n'⌝ ∗ ⌜C_p' ## C_m'⌝
+                         ∗ ⌜keyset K I_m' m ## keyset K I_n' n⌝
                          ∗ ⌜keyset K I_p' p ∪ keyset K I_n' n ∪ keyset K I_m' m = keyset K I_p p ∪ keyset K I_n n⌝ }}})%I.
 
   Parameter alloc_spec :
-      ({{{ True }}}
+     ⊢ ({{{ True }}}
            alloc #()
        {{{ (m: Node) (l:loc), RET #m; hrep_spatial m ∗ ⌜lockLoc m = l⌝ ∗ l ↦ #false }}})%I.
 
@@ -296,7 +257,7 @@ Section Coupling_Template.
           (lockLoc n) ↦ #b
           ∗ if b then True
             else (∃ (I_n: inset_flowint_ur K) (C_n: gset K),
-                 own γ (◯ I_n) ∗ ⌜domm I_n = {[n]}⌝ ∗ node n root I_n C_n
+                 own γ (◯ I_n) ∗ ⌜domm I_n = {[n]}⌝ ∗ node root n I_n C_n
                  ∗ own γ_k (◯ prod (keyset K I_n n, C_n)))))
     )%I.
 
@@ -334,88 +295,36 @@ Section Coupling_Template.
   Proof.
     unfold flowint_update_P.
     case_eq (auth_auth_proj x); last first.
-    - intros H. iIntros "(% & ?)". iExFalso. done.
-    - intros p. intros H. case_eq p. intros q a Hp.
-      iIntros "[% Hown]". destruct H0 as [I' H0].
-      destruct H0. destruct H1. destruct H2. destruct H3.
+    - intros Hx. iIntros "(% & ?)". iExFalso. done.
+    - intros p. intros Hx. case_eq p. intros q a Hp.
+      iIntros "[HI' Hown]". iDestruct "HI'" as %HI'.
+      destruct HI' as [I' HI'].
+      destruct HI' as [Hagree [Hq [HIn [Hcontxl HIo]]]].
       iExists I'.
-      iSplit. iPureIntro. apply H3.
-      iSplit. iPureIntro. apply H4.
-      assert (Auth (auth_auth_proj x) (auth_frag_proj x) = x) as Hx.
+      iSplit. by iPureIntro.
+      iSplit. by iPureIntro.
+      assert (Auth (auth_auth_proj x) (auth_frag_proj x) = x) as Hdefx.
       { destruct x. reflexivity. }
       assert (x = (Auth (Some (1%Qp, to_agree(I'))) (I_n'))) as H'.
-      { rewrite <-Hx. rewrite H. rewrite <-H2. rewrite Hp. rewrite H1.
-       rewrite H0. reflexivity. }
-      assert (● I' = Auth (Some (1%Qp, to_agree(I'))) ε) as HI'. { reflexivity. }
-      assert (◯ I_n' = Auth ε I_n') as HIn'. { reflexivity. }
-      assert (ε ⋅ I_n' = I_n') as HeIn.
-      { rewrite /(⋅) /=. rewrite left_id. done. }
-      assert (Some (1%Qp, to_agree I') ⋅ None = Some (1%Qp, to_agree I')) as Hs.
-      { rewrite /(⋅) /=.
-        rewrite /(cmra_op (optionR (prodR fracR (agreeR (inset_flowint_ur K)))) (Some (1%Qp, to_agree I')) (None)) /=.
-        reflexivity. }
-      assert (● I' ⋅ ◯ I_n' = (Auth (Some (1%Qp, to_agree(I'))) (I_n'))) as Hd.
-      { rewrite /(● I') /= /(◯ I_n') /=. rewrite /(⋅) /=.
-        rewrite /(cmra_op (authR (inset_flowint_ur K)) (Auth (Some (1%Qp, to_agree I')) ε) (Auth None I_n')) /=.
-        rewrite /auth_op /=. rewrite HeIn. rewrite Hs. reflexivity. }
-      iEval (rewrite Hd). iEval (rewrite <- H'). done.
+      { rewrite <-Hdefx. by rewrite Hx Hp Hq Hagree HIn. }
+      iEval (rewrite -auth_both_op). by iEval (rewrite <-H').
   Qed.
 
-
-  (** Lock module proofs *)
-
-  Lemma lockNode_spec (n: Node):
-    <<< ∀ (b: bool), (lockLoc n) ↦ #b >>>
-        lockNode #n    @ ⊤
-    <<< (lockLoc n) ↦ #true ∗ if b then False else True, RET #() >>>. (* rewrite if then else *)
-  Proof.
-    iIntros (Φ) "AU". iLöb as "IH".
-    wp_lam. wp_bind(getLockLoc _)%E.
-    wp_apply getLockLoc_spec; first done.
-    iIntros (l) "#Hl". wp_let. wp_bind (CmpXchg _ _ _)%E.
-    iMod "AU" as (b) "[Hb HAU]". iDestruct "Hl" as %Hl.
-    iEval (rewrite Hl) in "Hb". destruct b.
-    - wp_cmpxchg_fail. iDestruct "HAU" as "[HAU _]".
-      iEval (rewrite Hl) in "HAU".
-      iMod ("HAU" with "Hb") as "H".
-      iModIntro. wp_pures. iApply "IH".
-      iEval (rewrite <-Hl) in "H". done.
-    - wp_cmpxchg_suc. iDestruct "HAU" as "[_ HAU]".
-      iEval (rewrite Hl) in "HAU".
-      iMod ("HAU" with "[Hb]") as "HΦ". iFrame; done.
-      iModIntro. wp_pures. done.
-  Qed.
-
-  Lemma unlockNode_spec (n: Node) :
-          <<< lockLoc n ↦ #true >>>
-                unlockNode #n    @ ⊤
-          <<< lockLoc n ↦ #false, RET #() >>>.
-  Proof.
-    iIntros (Φ) "AU". wp_lam. wp_bind(getLockLoc _)%E.
-    wp_apply getLockLoc_spec; first done.
-    iIntros (l) "#Hl". wp_let.
-    iMod "AU" as "[Hy [_ Hclose]]".
-    iDestruct "Hl" as %Hl.
-    iEval (rewrite Hl) in "Hy".
-    wp_store. iEval (rewrite Hl) in "Hclose".
-    iMod ("Hclose" with "Hy") as "HΦ".
-    iModIntro. done.
-  Qed.
 
   (** Proof of the lock-coupling template *)
 
   Lemma traverse_spec (γ γ_fp γ_k γ_c: gname) (root: Node) (k: K) (p n: Node) (Ns: gset Node) I_p C_p I_n C_n:
-    ⌜k ∈ KS⌝ ∗ css γ γ_fp γ_k γ_c root -∗
+    ⊢ ⌜k ∈ KS⌝ ∗ css γ γ_fp γ_k γ_c root -∗
     {{{ own γ_fp (◯ Ns) ∗ ⌜p ∈ Ns⌝ ∗ ⌜n ∈ Ns⌝ ∗ ⌜root ∈ Ns⌝ ∗ ⌜n ≠ root⌝
-        ∗ node p root I_p C_p ∗ own γ (◯ I_p) ∗ ⌜domm I_p = {[p]}⌝ ∗  ⌜in_inset K k I_p p⌝ ∗ ⌜in_outset K k I_p n⌝
-        ∗ own γ_k (◯ prod (keyset K I_p p, C_p)) ∗ node n root I_n C_n ∗ own γ (◯ I_n) ∗ ⌜domm I_n = {[n]}⌝
+        ∗ node root p I_p C_p ∗ own γ (◯ I_p) ∗ ⌜domm I_p = {[p]}⌝ ∗  ⌜in_inset K k I_p p⌝ ∗ ⌜in_outset K k I_p n⌝
+        ∗ own γ_k (◯ prod (keyset K I_p p, C_p)) ∗ node root n I_n C_n ∗ own γ (◯ I_n) ∗ ⌜domm I_n = {[n]}⌝
         ∗ own γ_k (◯ prod (keyset K I_n n, C_n))
     }}}
       traverse #p #n #k @ ⊤
     {{{ (p' n': Node) (Ns': gsetUR Node) (I_p' I_n': inset_flowint_ur K) (C_p' C_n': gset K),
         RET (#p', #n');
         own γ_fp (◯ Ns') ∗ ⌜p' ∈ Ns'⌝ ∗ ⌜n' ∈ Ns'⌝ ∗ own γ (◯ I_p') ∗ ⌜domm I_p' = {[p']}⌝ ∗ own γ (◯ I_n')
-        ∗ ⌜domm I_n' = {[n']}⌝ ∗ node p' root I_p' C_p' ∗ node n' root I_n' C_n' ∗ ⌜n' ≠ root⌝
+        ∗ ⌜domm I_n' = {[n']}⌝ ∗ node root p' I_p' C_p' ∗ node root n' I_n' C_n' ∗ ⌜n' ≠ root⌝
         ∗ own γ_k (◯ prod (keyset K I_p' p', C_p'))
         ∗ own γ_k (◯ prod (keyset K I_n' n', C_n'))
         ∗ ⌜in_inset K k I_p' p'⌝ ∗ ⌜in_outset K k I_p' n'⌝ ∗ ⌜¬in_outsets K k I_n'⌝
@@ -425,7 +334,7 @@ Section Coupling_Template.
     iDestruct "H" as "(#Hfp & % & % & % & % & Hnodep & HIp & % & % & % & Hksp & Hnoden & HIn & % & Hksn)".
     wp_lam. wp_pures. wp_bind (findNext _ _)%E.
     iPoseProof ((own_op γ (◯ I_p) (◯ I_n)) with "[HIp HIn]") as "H"; first by eauto with iFrame.
-    iPoseProof (own_valid with "H") as "%". rewrite -auth_frag_op in H8.
+    iPoseProof (own_valid with "H") as "%". rewrite -auth_frag_op in H9.
     assert (✓ (I_p ⋅ I_n)). { apply (auth_frag_valid (◯ (I_p ⋅ I_n))). done. }
     assert (in_inset K k I_n n).
     { unfold in_inset. fold (inset K I_n n).
@@ -444,7 +353,7 @@ Section Coupling_Template.
       assert (✓ I0) as HI0. { apply (auth_auth_valid (I0)). done. }
       assert (n' ∈ domm I2). { apply (flowint_step I0 I_n I2 k n' root); try done. }
       assert (n' ∈ domm I0).
-      { rewrite H13. rewrite flowint_comp_fp. set_solver. rewrite <-H13. done. }
+      { rewrite H14. rewrite flowint_comp_fp. set_solver. rewrite <-H14. done. }
       iMod (own_update γ_fp (● (domm I0)) (● (domm I0) ⋅ ◯ (domm I0)) with "HFP") as "H".
       apply auth_update_core_id. apply gset_core_id. done.
       iDestruct "H" as "(HFP & #Hfp0)".
@@ -454,16 +363,18 @@ Section Coupling_Template.
       iAaccIntro with "Hlock". { iIntros "H". iModIntro. iFrame "∗ # %".
       iNext. iExists I0, C0. iFrame "∗ # %". iApply "Hstar".
       iExists b. iFrame "∗ # %". }
-      iIntros "(Hlock & H)". destruct b. { iExFalso. done. } iClear "H".
+      iIntros "(Hlock & H)". destruct b. { iDestruct "H" as %Ht.
+      pose proof (diff_false_true) as Hbeq. unfold not in Hbeq.
+      exfalso; apply Hbeq. rewrite Ht. done. } iClear "H".
       iDestruct "Hb" as (I_n' C_n') "(HIn' & % & Hnoden' & Hksn')".
       iPoseProof ((own_op γ (◯ I_n) (◯ I_n' )) with "[HIn HIn']") as "H"; first by eauto with iFrame.
-      iPoseProof (own_valid with "H") as "%". rewrite -auth_frag_op in H19.
+      iPoseProof (own_valid with "H") as "%". rewrite -auth_frag_op in H20.
       assert (✓ (I_n ⋅ I_n')). { apply (auth_frag_valid (◯ (I_n ⋅ I_n'))). done. }
       iEval (rewrite -auth_frag_op) in "H".
       iPoseProof ((auth_own_incl _ I0 _) with "[$HInt $H]") as (I3)"%".
-      iAssert (node n' root I_n' C_n' ∗ ⌜nodeinv root n' I_n' C_n'⌝)%I with "[Hnoden']" as "(Hnoden' & %)".
+      iAssert (node root n' I_n' C_n' ∗ ⌜nodeinv root n' I_n' C_n'⌝)%I with "[Hnoden']" as "(Hnoden' & %)".
       { iApply (node_implies_nodeinv _ _ _). iFrame "∗ # %". iPureIntro.
-        apply cmra_valid_op_r in H20. done. }
+        apply cmra_valid_op_r in H21. done. }
       assert (n' ≠ root) as Hnotf'.
       { apply (successor_not_root I0 I_n I_n' I3 C_n' root n' k); try done. }
       iModIntro. iSplitL "HKS HInt HFP Hcont Hstar Hlock".
@@ -473,21 +384,21 @@ Section Coupling_Template.
       iInv "HInv" as ">H". iDestruct "H" as (I1 C1) "(HKS & HInt & % & HFP & Hcont & Hstar)".
       iAssert (⌜p ∈ domm I1⌝)%I with "[HFP]" as "%".
       { iPoseProof ((auth_own_incl γ_fp (domm I1) (Ns)) with "[$]") as "%".
-        apply gset_included in H24.
+        apply gset_included in H25.
         iPureIntro. set_solver. }
       iAssert (⌜n ∈ domm I1⌝)%I with "[HFP]" as "%".
       { iPoseProof ((auth_own_incl γ_fp (domm I1) Ns) with "[$]") as "%".
-        apply gset_included in H25.
+        apply gset_included in H26.
         iPureIntro. set_solver. }
       iAssert (⌜n' ∈ domm I1⌝)%I with "[HFP]" as "%".
       { iPoseProof ((auth_own_incl γ_fp (domm I1)) with "[$]") as "%".
-        apply gset_included in H26.
+        apply gset_included in H27.
         iPureIntro. set_solver. }
       assert (root ∈ domm I1). { apply globalinv_root_fp. done. }
       rewrite (big_sepS_elem_of_acc _ (domm I1) p); last by eauto.
       iDestruct "Hstar" as "[Hb Hstar]". iDestruct "Hb" as (b) "[Hlock Hb]".
       destruct b; last first. { iDestruct "Hb" as (In1 Cn1) "(_ & _ & Hrep' & _)".
-      iAssert (⌜False⌝)%I with "[Hrep' Hnodep]" as %Hf. { iApply (node_sep_star p In1 I_p _ _ root).
+      iAssert (⌜False⌝)%I with "[Hrep' Hnodep]" as %Hf. { iApply (node_sep_star root p In1 I_p _ _).
       iFrame. } exfalso. done. }
       iAaccIntro with "Hlock". { iIntros. iModIntro. iFrame "∗ # %". iNext. iExists I1, C1.
       iFrame "∗ # %". iApply "Hstar". iExists true. iFrame. }
@@ -503,18 +414,11 @@ Section Coupling_Template.
       iApply "HCont". iFrame "∗ # %".
   Qed.
 
-  Lemma ghost_update_keyset γ_k dop k Cn Cn' res K1 C:
-    ⌜Ψ dop k Cn Cn' res⌝ ∗ own γ_k (● prod (KS, C)) ∗ own γ_k (◯ prod (K1, Cn))
-    ∗ ⌜Cn' ⊆ K1⌝ ∗ ⌜k ∈ K1⌝ ∗ ⌜k ∈ KS⌝
-    ==∗ ∃ C', ⌜Ψ dop k C C' res⌝ ∗ own γ_k (● prod (KS, C')) ∗ own γ_k (◯ prod (K1, Cn')).
-  Proof.
-  Admitted.
-    
   Theorem searchStrOp_spec (γ γ_fp γ_k γ_c: gname) root (k: K) (dop: dOp):
-    ⌜k ∈ KS⌝ ∗ css γ γ_fp γ_k γ_c root -∗
+    ⊢ ⌜k ∈ KS⌝ ∗ css γ γ_fp γ_k γ_c root -∗
     <<< ∀ (C: gset K), css_cont γ_c C >>>
       CSSOp dop root #k @ ⊤ ∖ ↑N
-    <<< ∃ C' (res: bool), css_cont γ_c C' ∗ ⌜Ψ dop k C C' res⌝, RET #res >>>.
+    <<< ∃ C' (res: bool), css_cont γ_c C' ∗ (Ψ dop k C C' res : iProp), RET #res >>>.
   Proof.
     iIntros "(% & #HInv)". iIntros (Φ) "AU". wp_lam. wp_bind (lockNode _)%E.
     awp_apply (lockNode_spec root). iInv "HInv" as ">H".
@@ -529,23 +433,27 @@ Section Coupling_Template.
     iAaccIntro with "Hlock". { iIntros "H". iModIntro. iSplitR "AU".
     iNext. iExists I0, C0. iFrame "∗ # %". iApply "Hstar".
     iExists b. iFrame "∗ # %". done. }
-    iIntros "(Hlock & H)". destruct b. { iExFalso. done. } iClear "H".
+    iIntros "(Hlock & H)". destruct b. { iDestruct "H" as %Ht.
+    pose proof (diff_false_true) as Hbeq. unfold not in Hbeq.
+    exfalso; apply Hbeq. rewrite Ht. done. } iClear "H".
     iDestruct "Hb" as (If Cf) "(HIf & % & Hnodef & HCf)".
     iPoseProof ((auth_own_incl _ I0) with "[$HInt $HIf]") as (Io)"%".
-    iModIntro. iSplitR "AU HIf Hnodef HCf". iNext. iExists I0, C0. iFrame "∗ # %".
+    iModIntro. iSplitR "AU HIf Hnodef HCf". iNext.
+    iExists I0, C0. iFrame "∗ # %".
     iApply "Hstar". iExists true. iFrame "∗ # %".
     wp_pures. wp_bind(findNext _ _)%E.
-    assert (in_inset K k If root). { unfold globalinv in H0. destruct H0 as [? [? [? ?]]].
-    specialize (H6 root). destruct H6 as [H6 _]. apply (inset_monotone I0 If Io k root); try done; set_solver. }
+    assert (in_inset K k If root). { unfold globalinv in H1. destruct H1 as [? [? [? ?]]].
+    specialize (H7 root). destruct H7 as [H7 _]. apply (inset_monotone I0 If Io k root); try done; set_solver. }
     wp_apply ((findNext_spec root root If Cf k) with "[Hnodef]").
     { iFrame "∗ # %". } iIntros (b n) "(Hnodef & Hb)".
     destruct b; last first. wp_pures. iDestruct "Hb" as "(% & %)".
-    exfalso. apply H5. done. iDestruct "Hb" as "%". wp_pures.
+    exfalso. apply H6. done. iDestruct "Hb" as "%". wp_pures.
     wp_bind (lockNode _)%E. awp_apply (lockNode_spec n). iInv "HInv" as ">H".
     iDestruct "H" as (I2 C2) "(HKS & HInt & % & HFP & Hcont & Hstar)".
     iPoseProof (own_valid with "HInt") as "%". rename H7 into Hcheck.
     assert (✓ I2) as HI2. { apply (auth_auth_valid (I2)). done. }
-    iPoseProof ((auth_own_incl _ I2) with "[$HInt $HIf]") as (Io')"%". assert (n ∈ domm I2).
+    iPoseProof ((auth_own_incl _ I2) with "[$HInt $HIf]") as (Io')"%".
+    assert (n ∈ domm I2).
     { assert (n ∈ domm Io').
       { apply (flowint_step I2 If Io' k n root); try done. }
       rewrite H7. rewrite flowint_comp_fp. set_solver. rewrite <-H7. done. }
@@ -555,19 +463,21 @@ Section Coupling_Template.
     iAaccIntro with "Hlock". { iIntros "H". iModIntro. iSplitR "AU HIf HCf Hnodef".
     iNext. iExists I2, C2. iFrame "∗ # %". iApply "Hstar".
     iExists b. iFrame "∗ # %". iFrame "∗ # %". }
-    iIntros "(Hlock & H)". destruct b. { iExFalso. done. } iClear "H".
+    iIntros "(Hlock & H)". destruct b. { iDestruct "H" as %Ht.
+    pose proof (diff_false_true) as Hbeq. unfold not in Hbeq.
+    exfalso; apply Hbeq. rewrite Ht. done. } iClear "H".
     assert (root ∈ domm I2). { apply globalinv_root_fp. done. }
     iMod (own_update γ_fp (● (domm I2)) (● (domm I2) ⋅ ◯ (domm I2)) with "HFP") as "H".
     apply auth_update_core_id. apply gset_core_id. done.
     iDestruct "H" as "(HFP & #Hfp2)".
     iDestruct "Hb" as (In Cn) "(HIn & % & Hnoden & HCn)".
     iPoseProof ((own_op γ (◯ If) (◯ In)) with "[HIf HIn]") as "H"; first by eauto with iFrame.
-    iPoseProof (own_valid with "H") as "%". rewrite -auth_frag_op in H11.
+    iPoseProof (own_valid with "H") as "%". rewrite -auth_frag_op in H12.
     assert (✓ (If ⋅ In)). { apply (auth_frag_valid (◯ (If ⋅ In))). done. }
     iEval (rewrite -auth_frag_op) in "H".
     iPoseProof ((auth_own_incl _ I2) with "[$HInt $H]") as (Iu)"%".
-    iAssert (node n root In Cn ∗ ⌜nodeinv root n In Cn⌝)%I with "[Hnoden]" as "(Hnoden & %)".
-    { iApply (node_implies_nodeinv n In Cn root). iFrame "∗ # %". iPureIntro.
+    iAssert (node root n In Cn ∗ ⌜nodeinv root n In Cn⌝)%I with "[Hnoden]" as "(Hnoden & %)".
+    { iApply (node_implies_nodeinv root n In Cn). iFrame "∗ # %". iPureIntro.
       apply cmra_valid_op_r in H12. done. }  iDestruct "H" as "(HIf & HIn)".
     assert (n ≠ root).
     { apply (successor_not_root I2 If In Iu Cn root n k); try done. }
@@ -585,7 +495,7 @@ Section Coupling_Template.
     iDestruct "H" as (I3 C3) "(HKS & HInt & % & HFP & Hcont & Hstar)".
     destruct (decide (m ∈ domm I3)). { rewrite (big_sepS_elem_of_acc _ (domm I3) m); last by eauto.
     iDestruct "Hstar" as "(Hm & Hstar)". iDestruct "Hm" as (b) "(Hlockm & Hb)".
-    iEval (rewrite H24) in "Hlockm". iDestruct (mapsto_valid_2 with "Hlm Hlockm") as "%".
+    iEval (rewrite H25) in "Hlockm". iDestruct (mapsto_valid_2 with "Hlm Hlockm") as "%".
     exfalso. done. }
     assert (root ∈ domm I3). { apply globalinv_root_fp. done. }
     assert (m ≠ root). { set_solver. }
@@ -593,99 +503,114 @@ Section Coupling_Template.
     iExists I3, C3. iFrame "∗ # %". iModIntro.
     wp_apply ((decisiveOp_insert_spec dop root p' n' m k Ip' In' Cp' Cn')
           with "[Hnodep' Hnoden' Hrepm]"). { iFrame "∗ % #". }
-    iIntros (Cp'' Cn'' Cm'' Ip'' In'' Im'' res) "(Hnodep' & Hnoden' & Hnodem' & % & % & Hminf & H)".
-    iDestruct "H" as "(% & % & % & % & % & % & % & % & % & % & % & % & %)".
-    iDestruct "Hminf" as "%". rename H43 into Hminf. 
+    iIntros (Cp'' Cn'' Cm'' Ip'' In'' Im'' res) "(Hnodep' & Hnoden' & Hnodem' & #HΨ & % & Hminf & H)".
+    iDestruct "H" as "(% & % & % & % & % & % & %)".
+    iDestruct "Hminf" as %Hminf. 
     iApply fupd_wp. iInv "HInv" as ">H".
     iDestruct "H" as (I4 C4) "(HKS & HInt & % & HFP & Hcont & Hstar)".
     iMod "AU" as (C') "[Hc [_ Hclose]]". iEval (rewrite /css_cont) in "Hc".
     iDestruct (auth_agree with "Hcont Hc") as %<-.
 
     (* ------ keyset update -------*)
-
+    
+    iAssert (⌜Cp'' ⊆ keyset K Ip'' p'⌝)%I with "[Hnodep']" as "%".
+    { iPoseProof (node_implies_nodeinv with "[Hnodep']") as "H". iFrame.
+      iPureIntro. unfold contextualLeq in H29. destruct H29 as [_ [H29 _]].
+      by repeat apply cmra_valid_op_l in H29. iDestruct "H" as "(_ & %)".
+      unfold nodeinv in H38. destruct H38 as [_ [H38 ]]. by iPureIntro. } 
+    iAssert (⌜Cn'' ⊆ keyset K In'' n'⌝)%I with "[Hnoden']" as "%".
+    { iPoseProof (node_implies_nodeinv with "[Hnoden']") as "H". iFrame.
+      iPureIntro. unfold contextualLeq in H29. destruct H29 as [_ [H29 _]].
+      apply cmra_valid_op_l in H29. by apply cmra_valid_op_r in H29.
+      iDestruct "H" as "(_ & %)". unfold nodeinv in H39.
+      destruct H39 as [_ [H39 ]]. by iPureIntro. } 
+    iAssert (⌜Cm'' ⊆ keyset K Im'' m⌝)%I with "[Hnodem']" as "%".
+    { iPoseProof (node_implies_nodeinv with "[Hnodem']") as "H". iFrame.
+      iPureIntro. unfold contextualLeq in H29. destruct H29 as [_ [H29 _]].
+      by repeat apply cmra_valid_op_r in H29. iDestruct "H" as "(_ & %)".
+      unfold nodeinv in H40. destruct H40 as [_ [H40 ]]. by iPureIntro. }
+    assert (Cp'' ## Cn''). { clear -H38 H39 H33. set_solver. }
+    assert (Cn'' ## Cm''). { clear -H40 H39 H35. set_solver. }
+    assert (Cm'' ## Cp''). { clear -H38 H40 H34. set_solver. }
     iPoseProof ((own_op γ_k (◯ prod (keyset K Ip' p', Cp')) (◯ prod (keyset K In' n', Cn'))
                       with "[Hksp' Hksn']")) as "H"; first by eauto with iFrame.
-    assert (◯ prod (keyset K Ip' p', Cp') ⋅ ◯ prod (keyset K In' n', Cn') =
-               ◯ (prod (keyset K Ip' p', Cp') ⋅ prod (keyset K In' n', Cn'))).
-    { apply (auth_frag_op (prod (keyset K Ip' p', Cp')) (prod (keyset K In' n', Cn'))). }
-    iEval (rewrite H44) in "H". iPoseProof (own_valid with "H") as "%".
-    assert (✓ (prod (keyset K Ip' p', Cp') ⋅ prod (keyset K In' n', Cn'))).
-    { apply (auth_frag_valid (◯ (prod (keyset K Ip' p', Cp') ⋅ prod (keyset K In' n', Cn')))). done. }
-    unfold op,prodOp in H46. repeat case_decide;
+    iEval (rewrite -auth_frag_op) in "H".
+    iPoseProof (own_valid with "H") as "%".
+    rewrite auth_frag_valid in H44 *; intros Hvprod.
+    unfold op, cmra_op in Hvprod. simpl in Hvprod. unfold ucmra_op in Hvprod.
+    simpl in Hvprod. repeat case_decide;
         [ simpl | try exfalso; eauto | try exfalso; eauto | try exfalso; eauto | try exfalso; eauto].
     assert (prod (keyset K Ip'' p', Cp'') ⋅ prod (keyset K In'' n', Cn'') ⋅ prod (keyset K Im'' m, Cm'')
                  = prod (keyset K Ip'' p' ∪ keyset K In'' n' ∪ keyset K Im'' m, Cp'' ∪ Cn'' ∪ Cm'')).
-    { unfold op, prodOp. repeat case_decide; try done. exfalso. apply H58. set_solver by eauto.
-      exfalso. apply H57. set_solver by eauto. exfalso. apply H55. set_solver by eauto. }
+    { unfold op, prodOp. repeat case_decide; try done. exfalso. apply H55. set_solver by eauto.
+      exfalso. apply H54. clear - H33 H34 H35. set_solver by eauto. exfalso. apply H52. set_solver by eauto. }
     assert (◯ (prod (keyset K Ip'' p', Cp'') ⋅ prod (keyset K In'' n', Cn'') ⋅ prod (keyset K Im'' m, Cm''))
                  = ◯ (prod (keyset K Ip'' p' ∪ keyset K In'' n' ∪ keyset K Im'' m, Cp'' ∪ Cn'' ∪ Cm''))).
-    { rewrite H51. reflexivity. }
+    { rewrite H48. reflexivity. }
     assert ((prod (keyset K Ip' p', Cp') ⋅ prod (keyset K In' n', Cn'))
                   = prod (keyset K Ip' p' ∪ keyset K In' n', Cp' ∪ Cn')).
     { unfold op, prodOp. repeat case_decide; try done. }
     iPoseProof ((own_op γ (◯ Ip') (◯ In')) with "[HIp' HIn']") as "H'"; first by eauto with iFrame.
-    iPoseProof (own_valid with "H'") as "%". rewrite -auth_frag_op in H54.
+    iPoseProof (own_valid with "H'") as "%". rewrite -auth_frag_op in H51.
     assert (✓ (Ip' ⋅ In')). { apply (auth_frag_valid (◯ (Ip' ⋅ In'))). done. }
     assert (in_inset K k In' n'). {
-      apply (flowint_inset_step Ip' In' k n'); try done. set_solver. }
+      apply (flowint_inset_step Ip' In' k n'); try done. rewrite H20. clear. set_solver. }
     assert (k ∈ keyset K In' n'). { apply keyset_def; try done. }
     iMod ((ghost_update_keyset γ_k dop k (Cp' ∪ Cn') (Cp'' ∪ Cn'' ∪ Cm'') res
                  (keyset K Ip' p' ∪ keyset K In' n') C4) with "[HKS H]") as "Hgks".
-    iEval (rewrite H53) in "H". iFrame "∗ # %". iPureIntro.
-    split. rewrite <-H42. set_solver by eauto. set_solver by eauto.
-    iDestruct "Hgks" as (C4') "(% & HKS & H)". iEval (rewrite <-H42) in "H".
+    iEval (rewrite H50) in "H". iFrame "∗ # %". iPureIntro.
+    split. rewrite <-H36. clear -H38 H39 H40. set_solver. clear -H54. set_solver.
+    iDestruct "Hgks" as (C4') "(#HΨ' & HKS & H)". iEval (rewrite <-H36) in "H".
     iAssert (own γ_k (◯ (prod (keyset K Ip'' p', Cp'') ⋅ prod (keyset K In'' n', Cn'') ⋅ prod (keyset K Im'' m, Cm''))))
-          with "[H]" as "Hv". { iEval (rewrite H52). done. }
+          with "[H]" as "Hv". { iEval (rewrite H48). done. }
     iDestruct "Hv" as "((Hksp' & Hksn') & Hksm')".
     iMod (auth_excl_update γ_c (C4') with "Hcont Hc") as "[Hcont Hc]".
-    clear H51 H52 H53 H44 H45 H47 H48 H49 H50 H46 H51 H33 H34 H35 H36 H37.
-    clear H38 H39 H40 H41 H42 H0 H1 H2 H3 H4 H5 H6 Hcheck HI2 H7 H8 H9 H10.
-    clear H11 H12 H13 H14 H15 H25 n0 H26 C0 If Cf n C2 Io' In Cn 
-    Iu I3 C3.
-
+    clear - H0 node_implies_nodeinv node_sep_star p' n' Ns Ip' In' Cp'
+            Cn' H17 H18 H19 H20 H21 H22 H23 H24 m lm H25 Cp'' Cn'' Cm'' Ip''
+            In'' Im'' res H29 H30 H31 H32 Hminf I4 C4 H37 H51 H52 H53 H54 C4'.
 
     (* ------ interface update -------*)
 
     destruct (decide (m ∈ domm I4)). { rewrite (big_sepS_elem_of_acc _ (domm I4) m); last by eauto.
     iDestruct "Hstar" as "(Hm & Hstar)". iDestruct "Hm" as (b) "(Hlockm & Hb)".
-    iEval (rewrite H24) in "Hlockm". iDestruct (mapsto_valid_2 with "Hlm Hlockm") as "%".
+    iEval (rewrite H25) in "Hlockm". iDestruct (mapsto_valid_2 with "Hlm Hlockm") as "%".
     exfalso. done. }
     assert (◯ Ip' ⋅ ◯ In' = ◯ (Ip' ⋅ In')).
-    by rewrite auth_frag_op. iEval (rewrite H0) in "H'". iCombine "HInt" "H'" as "Hownint".
+    by rewrite auth_frag_op. iEval (rewrite H1) in "H'". iCombine "HInt" "H'" as "Hownint".
     iPoseProof (own_valid with "Hownint") as "%".
-    apply auth_both_valid in H1. destruct H1. destruct H1 as [Iz H1].
+    apply auth_both_valid in H2. destruct H2. destruct H2 as [Iz H2].
     iDestruct "Hownint" as "[HInt H']".
     destruct H29 as (Hvldpn & Hvldpnm & Hsub & Hinf & Hout).
     assert (domm (Ip'' ⋅ In'' ⋅ Im'') = domm Ip'' ∪ domm In'' ∪ domm Im''). 
     repeat rewrite (flowint_comp_fp); try done. by apply cmra_valid_op_l in Hvldpnm.
-    rewrite H30 in H3. rewrite H31 in H3. rewrite H32 in H3.
-    assert (m ∉ domm Iz). { apply leibniz_equiv in H1. rewrite H1 in n.
-    rewrite (flowint_comp_fp) in n. set_solver. apply leibniz_equiv_iff in H1.
-    rewrite <-H1. done. }
-    unfold globalinv in H43. destruct H43 as (Hv & H4root & H4out & H4in).
+    rewrite H30 H31 H32 in H4.
+    assert (m ∉ domm Iz). { apply leibniz_equiv in H2. rewrite H2 in n.
+    rewrite (flowint_comp_fp) in n. set_solver. apply leibniz_equiv_iff in H2.
+    rewrite <-H2. done. }
+    unfold globalinv in H37. destruct H37 as (Hv & H4root & H4out & H4in).
     assert (out Iz m = 0%CCM).
     { 
-      apply (intComp_out_zero (Ip'⋅In') Iz m). by rewrite <-H1.
-      rewrite <-H1. done. rewrite <-H1. apply nzmap_eq.
+      apply (intComp_out_zero (Ip'⋅In') Iz m). by rewrite <-H2.
+      rewrite <-H2. done. rewrite <-H2. apply nzmap_eq.
       intros km. pose proof (H4out km m).
-      unfold outset, dom_ms in H5. rewrite (nzmap_elem_of_dom_total) in H5 *; intros.
-      apply dec_stable in H5. rewrite H5.
+      unfold outset, dom_ms in H6. rewrite (nzmap_elem_of_dom_total) in H6 *; intros.
+      apply dec_stable in H6. rewrite H6.
       by rewrite nzmap_lookup_empty.
     }    
     iMod (own_updateP (flowint_update_P K_multiset I4 (Ip' ⋅ In') (Ip'' ⋅ In'' ⋅ Im'')) γ
                           (● I4 ⋅ ◯ (Ip' ⋅ In')) with "[HInt H']") as (Io'') "H0".
     {
-      rewrite H1.
+      rewrite H2.
       apply (flowint_update K_multiset (Iz) (Ip' ⋅ In') (Ip'' ⋅ In'' ⋅ Im'')).
-      repeat split; try done. apply leibniz_equiv in H1. assert (H4valid := H2).
-      rewrite H1 in H2. apply intComposable_valid in H2. unfold intComposable in H2.
-      destruct H2 as (_ & _ & Hdisj & _). rewrite flowint_comp_fp in Hdisj; last first.
-      rewrite H1 in H4valid; by apply cmra_valid_op_l in H4valid.
-      rewrite H3. rewrite H18 in Hdisj. rewrite H19 in Hdisj. set_solver.
+      repeat split; try done. apply leibniz_equiv in H2. assert (H4valid := H3).
+      rewrite H2 in H3. apply intComposable_valid in H3. unfold intComposable in H3.
+      destruct H3 as (_ & _ & Hdisj & _). rewrite flowint_comp_fp in Hdisj; last first.
+      rewrite H2 in H4valid; by apply cmra_valid_op_l in H4valid.
+      rewrite H4. rewrite H19 H20 in Hdisj. clear -Hdisj H5. set_solver.
       intros nf. rewrite flowint_comp_fp; try done. 
       repeat rewrite (flowint_comp_fp); last by apply cmra_valid_op_l in Hvldpnm.
-      rewrite H30 H31 H32 H18 H19. intros Hnf. assert (nf = m). set_solver. replace nf.
-      unfold out in H5. done. done.
+      rewrite H30 H31 H32 H19 H20. intros Hnf. assert (nf = m). set_solver. replace nf.
+      unfold out in H6. done. done.
     }
     { try repeat rewrite own_op; iFrame. }
     iPoseProof ((flowint_update_result γ I4 (Ip' ⋅ In') (Ip'' ⋅ In'' ⋅ Im''))
@@ -704,7 +629,7 @@ Section Coupling_Template.
     iDestruct "HIpn''" as "(HIp'' & HIn'')".
     destruct (decide (m ∈ domm I4)). { rewrite (big_sepS_elem_of_acc _ (domm I4) m); last by eauto.
     iDestruct "Hstar" as "(Hm & Hstar)". iDestruct "Hm" as (b) "(Hlockm & Hb)".
-    iEval (rewrite H24) in "Hlockm". iDestruct (mapsto_valid_2 with "Hlm Hlockm") as "%".
+    iEval (rewrite H25) in "Hlockm". iDestruct (mapsto_valid_2 with "Hlm Hlockm") as "%".
     exfalso. done. }
     iMod (own_update γ_fp (● domm I4) (● (domm I4 ∪ {[m]}) ⋅ ◯ (domm I4 ∪ {[m]})) with "[HFP]") as "H".
     { apply (auth_update_alloc (domm I4) (domm I4 ∪ {[m]}) (domm I4 ∪ {[m]})).
@@ -712,18 +637,17 @@ Section Coupling_Template.
     done. iDestruct "H" as "(HFP & #Hfp4)".
     assert (domm I' = domm I4 ∪ {[m]}).
     {
-      destruct H7 as [I_o H7]. destruct H7.
+      destruct H8 as [I_o H8]. destruct H8.
       assert (domm I' = {[p']} ∪ {[n']} ∪ {[m]} ∪ domm I_o).
       {
         subst I'. repeat rewrite flowint_comp_fp; try congruence; try done.
         by apply (auth_auth_valid).
       }
-      rewrite H12.
       assert (domm I4 = {[p']} ∪ {[n']} ∪ domm I_o).
       {
         subst I4. repeat rewrite flowint_comp_fp; try congruence; try done.
       }
-      rewrite H13.
+      rewrite H13 H14.
       clear. set_solver.
     }
     
@@ -732,32 +656,33 @@ Section Coupling_Template.
       all : trivial.
       unfold globalinv. repeat split; try done. apply H4in. apply H4in.
       intros.
-      assert (n1 = m). { clear - H12 n0 H11. set_solver. } subst n1.
+      assert (n1 = m). { clear - H12 n0 H13. set_solver. } subst n1.
       unfold inset. unfold dom_ms. unfold inf. case_eq (inf_map I' !! m); last first.
       - intros Hm. unfold ccmunit, ccm_unit. simpl. unfold nzmap_dom. simpl. set_solver.
-      - intros k0 Hk0. simpl. destruct H7 as [Iz' [H7 ?]]. 
-        rewrite H7 in H1. apply intComp_cancelable in H1; last by rewrite H7 in H2.
-        apply leibniz_equiv in H1. subst Iz'.
+      - intros k0 Hk0. simpl. destruct H8 as [Iz' [H8 ?]]. 
+        rewrite H8 in H2. apply intComp_cancelable in H2; last by rewrite H8 in H3.
+        apply leibniz_equiv in H2. subst Iz'.
         assert (inf (Ip'' ⋅ In'' ⋅ Im'' ⋅ Iz) m = (inf (Ip'' ⋅ In''⋅ Im'') m) - (out Iz m))%CCM.
-        { apply intComp_inf_1. apply leibniz_equiv_iff in H13. rewrite <-H13.
+        { apply intComp_inf_1. apply leibniz_equiv_iff in H14. rewrite <-H14.
           by apply auth_auth_valid.
           assert (domm (Ip'' ⋅ In'' ⋅ Im'') = domm Ip'' ∪ domm In'' ∪ domm Im''). 
-          repeat rewrite (flowint_comp_fp); try done. rewrite H1.
+          repeat rewrite (flowint_comp_fp); try done. rewrite H2.
           rewrite H32. clear. set_solver.
         }
-        rewrite Hminf in H1. rewrite <-H13 in H1.
-        rewrite H5 in H1. rewrite ccm_pinv_unit in H1. unfold inf in H1. rewrite Hk0 in H1.
-        simpl in H1. rewrite H1. unfold ccmunit, lift_unit, nzmap_unit. simpl.
+        rewrite Hminf in H2. rewrite <-H14 in H2.
+        rewrite H6 in H2. rewrite ccm_pinv_unit in H2. unfold inf in H2. rewrite Hk0 in H2.
+        simpl in H2. rewrite H2. unfold ccmunit, lift_unit, nzmap_unit. simpl.
         unfold nzmap_dom. simpl. set_solver.
     }
-    iEval (rewrite <-H11) in "HFP". assert (domm I'∖ {[m]} = domm I4). { set_solver. }
+    iEval (rewrite <-H12) in "HFP". assert (domm I'∖ {[m]} = domm I4). 
+    { clear -n0 H12. set_solver. }
 
     (* ------ updates over -------*)
 
     iMod ("Hclose" with "[Hc]") as "HΦ". iFrame "∗ % #".
     iModIntro. iSplitL "Hstar Hlm Hnodem' HKS Hcont HI' HIm'' HFP Hksm'". iNext. iExists I', C4'.
-    iFrame "∗ # %". rewrite (big_sepS_delete _ (domm I') m); last set_solver. iEval (rewrite H13).
-    iFrame. iExists false. iEval (rewrite H24). iFrame. iExists Im'', Cm''. eauto with iFrame.
+    iFrame "∗ # %". rewrite (big_sepS_delete _ (domm I') m); last set_solver. iEval (rewrite H14).
+    iFrame. iExists false. iEval (rewrite H25). iFrame. iExists Im'', Cm''. eauto with iFrame.
     iModIntro. wp_pures. wp_bind (unlockNode _)%E.
 
     (* ------ linearization over -------*)
@@ -766,12 +691,12 @@ Section Coupling_Template.
     iDestruct "H" as (I6 C6) "(HKS & HInt & % & HFP & Hcont & Hstar)".
     iAssert (⌜p' ∈ domm I6⌝)%I with "[HFP]" as "%".
     { iPoseProof ((auth_own_incl γ_fp (domm I6) Ns) with "[$]") as "%".
-      apply gset_included in H15.
-      iPureIntro. clear -H15 H16. set_solver. }
+      apply gset_included in H16.
+      iPureIntro. clear -H16 H17. set_solver. }
     rewrite (big_sepS_elem_of_acc _ (domm I6) p'); last by eauto.
     iDestruct "Hstar" as "[Hb Hstar]". iDestruct "Hb" as (b) "[Hlock Hb]".
     destruct b; last first. { iDestruct "Hb" as (In0 Cn0) "(_ & _ & Hrep' & _)".
-    iAssert (⌜False⌝)%I with "[Hnodep' Hrep']" as %Hf. { iApply (node_sep_star p' Ip'' In0 _ _ _).
+    iAssert (⌜False⌝)%I with "[Hnodep' Hrep']" as %Hf. { iApply (node_sep_star root p' Ip'' In0 _ _).
     iFrame. } exfalso. done. }
     iAaccIntro with "Hlock". 
     { iIntros. iModIntro. iFrame "∗". iNext. iExists I6, C6.
@@ -786,12 +711,12 @@ Section Coupling_Template.
     iInv "HInv" as ">H". iDestruct "H" as (I7 C7) "(HKS & HInt & % & HFP & Hcont & Hstar)".
     iAssert (⌜n' ∈ domm I7⌝)%I with "[HFP]" as "%".
     { iPoseProof ((auth_own_incl γ_fp (domm I7) Ns) with "[$]") as "%".
-      apply gset_included in H26.
-      iPureIntro. clear -H26 H17. set_solver. }
+      apply gset_included in H27.
+      iPureIntro. clear -H18 H27. set_solver. }
     rewrite (big_sepS_elem_of_acc _ (domm I7) n'); last by eauto.
     iDestruct "Hstar" as "[Hb Hstar]". iDestruct "Hb" as (b) "[Hlock Hb]".
     destruct b; last first. { iDestruct "Hb" as (In0 Cn0) "(_ & _ & Hrep' & _)".
-    iAssert (⌜False⌝)%I with "[Hnoden' Hrep']" as %Hf. { iApply (node_sep_star n' In'' In0 _ _ _).
+    iAssert (⌜False⌝)%I with "[Hnoden' Hrep']" as %Hf. { iApply (node_sep_star root n' In'' In0 _ _).
     iFrame. } exfalso. done. }
     iAaccIntro with "Hlock".
     { iIntros. iModIntro. iFrame "∗ # %". iNext. iExists I7, C7.
